Use bytes interface without index notion

MLS.Parser.fst
@@ -1,24 +1,24 @@
 module MLS.Parser
 
-module IT = Lib.IntTypes
-open Lib.ByteSequence
+open MLS.Bytes
 
 #set-options "--fuel 0 --ifuel 2"
 
 (*** Helper functions ***)
 
 let delete_prefix (b:bytes) (i:consumed_length b) : bytes =
-  Seq.slice b i (Seq.length b)
+  bytes_slice b i (bytes_length b)
 
 val delete_prefix_length: b:bytes -> i:consumed_length b -> Lemma
-  (Seq.length (delete_prefix b i) == (Seq.length b) - i)
-  [SMTPat (Seq.length (delete_prefix b i))]
-let delete_prefix_length b i = ()
+  (bytes_length (delete_prefix b i) == (bytes_length b) - i)
+  [SMTPat (bytes_length (delete_prefix b i))]
+let delete_prefix_length b i =
+  bytes_slice_length b i (bytes_length b)
 
-val delete_prefix_index: b:bytes -> i:consumed_length b -> j:nat{j < Seq.length (delete_prefix b i)} -> Lemma
-  (Seq.index (delete_prefix b i) j == Seq.index b (j+i))
-  [SMTPat (Seq.index (delete_prefix b i) j)]
-let delete_prefix_index b i j = ()
+//val delete_prefix_index: b:bytes -> i:consumed_length b -> j:nat{j < bytes_length (delete_prefix b i)} -> Lemma
+//  (bytes_index (delete_prefix b i) j == bytes_index b (j+i))
+//  [SMTPat (bytes_index (delete_prefix b i) j)]
+//let delete_prefix_index b i j = ()
 
 (*** Parser combinators ***)
 
@@ -35,7 +35,7 @@ let bind #a #b ps_a ps_b =
   in
   let serialize_ab (x:(xa:a&(b xa))): bytes =
     let (|xa, xb|) = x in
-    Seq.append (ps_a.serialize xa) ((ps_b xa).serialize xb)
+    bytes_concat (ps_a.serialize xa) ((ps_b xa).serialize xb)
   in
   let lemma_not_unit (): Lemma((parse_ab bytes_empty == None) <==> (ps_a.parse bytes_empty == None) \/ (forall xa. (ps_b xa).parse bytes_empty == None)) = begin
     match parse_ab bytes_empty with
@@ -44,13 +44,38 @@ let bind #a #b ps_a ps_b =
       | None -> ()
       | Some (xa, la) ->
         FStar.Classical.forall_intro (fun (x:a) -> (
-          assert (Seq.equal (delete_prefix bytes_empty la) bytes_empty);
+          let lemma (): Lemma ((delete_prefix bytes_empty la) == bytes_empty) =
+            delete_prefix_length bytes_empty la;
+            bytes_empty_length ();
+            bytes_length_zero (delete_prefix bytes_empty la)
+          in lemma ();
           ps_a.parse_serialize_inv x;
+          let lemma (): Lemma (la == 0) =
+            bytes_empty_length ()
+          in lemma ();
+          let lemma (): Lemma (bytes_slice bytes_empty 0 la == bytes_empty) =
+            bytes_slice_length bytes_empty 0 la;
+            bytes_length_zero (bytes_slice bytes_empty 0 la)
+          in lemma ();
+          let lemma (): Lemma (bytes_slice (ps_a.serialize x) 0 la == bytes_empty) =
+            bytes_slice_length (ps_a.serialize x) 0 la;
+            bytes_length_zero (bytes_slice (ps_a.serialize x) 0 la)
+          in lemma ();
           ps_a.parse_no_lookahead bytes_empty (ps_a.serialize x);
           ()
         ) <: Lemma (is_not_unit (ps_b x)))
     end
-    | Some _ -> ()
+    | Some _ -> (
+      match ps_a.parse bytes_empty with
+      | None -> ()
+      | Some (xa, la) -> (
+        let lemma (): Lemma ((delete_prefix bytes_empty la) == bytes_empty) =
+          delete_prefix_length bytes_empty la;
+          bytes_empty_length ();
+          bytes_length_zero (delete_prefix bytes_empty la)
+        in lemma ()
+      )
+    )
   end in
   lemma_not_unit ();
   ({
@@ -58,10 +83,14 @@ let bind #a #b ps_a ps_b =
     serialize = serialize_ab;
     parse_serialize_inv = (fun (x:(xa:a&(b xa))) ->
       let (|xa, xb|) = x in
-      ps_a.parse_no_lookahead (ps_a.serialize xa) (serialize_ab x);
       ps_a.parse_serialize_inv xa;
       (ps_b xa).parse_serialize_inv xb;
-      assert (Seq.equal (delete_prefix (serialize_ab x) (Seq.length (ps_a.serialize xa))) ((ps_b xa).serialize xb))
+      bytes_concat_length (ps_a.serialize xa) ((ps_b xa).serialize xb);
+      bytes_slice_concat_left (ps_a.serialize xa) ((ps_b xa).serialize xb);
+      bytes_slice_concat_right (ps_a.serialize xa) ((ps_b xa).serialize xb);
+      bytes_slice_whole (ps_a.serialize xa);
+      ps_a.parse_no_lookahead (ps_a.serialize xa) (serialize_ab x);
+      ()
     );
     serialize_parse_inv = (fun (buf:bytes) ->
       match parse_ab buf with
@@ -71,19 +100,31 @@ let bind #a #b ps_a ps_b =
         let (xb, lb) = Some?.v ((ps_b xa).parse (delete_prefix buf la)) in
         ps_a.serialize_parse_inv buf;
         (ps_b xa).serialize_parse_inv (delete_prefix buf la);
-        assert (Seq.equal (Seq.slice buf 0 (la+lb)) (serialize_ab xab))
+        bytes_slice_slice buf la (bytes_length buf) 0 lb;
+        bytes_slice_slice buf 0 (la+lb) 0 la;
+        bytes_slice_slice buf 0 (la+lb) la (la+lb);
+        bytes_slice_length buf 0 (la+lb);
+        bytes_concat_slice (bytes_slice buf 0 (la+lb)) la
     );
     parse_no_lookahead = (fun (b1 b2:bytes) ->
       match parse_ab b1 with
       | None -> ()
       | Some (xab, l) ->
         let (|xa, xb|) = xab in
+        let (_, la) = Some?.v (ps_a.parse b1) in
+        bytes_slice_slice b1 0 l 0 la;
+        bytes_slice_slice b2 0 l 0 la;
         ps_a.parse_no_lookahead b1 b2;
-        let (_, la1) = Some?.v (ps_a.parse b1) in
-        let (_, la2) = Some?.v (ps_a.parse b2) in
-        (ps_b xa).parse_no_lookahead (delete_prefix b1 la1) (delete_prefix b2 la2)
+        let (_, lb1) = Some?.v ((ps_b xa).parse (delete_prefix b1 la)) in
+        bytes_slice_slice b1 la (bytes_length b1) 0 lb1;
+        bytes_slice_slice b2 la (bytes_length b2) 0 lb1;
+        bytes_slice_slice b1 0 (la + lb1) la (la+lb1);
+        bytes_slice_slice b2 0 (la + lb1) la (la+lb1);
+        (ps_b xa).parse_no_lookahead (delete_prefix b1 la) (delete_prefix b2 la);
+        ()
     )
   })
+
 
 let isomorphism_explicit #a b ps_a f g g_f_inv f_g_inv =
   let parse_b buf =
@@ -123,33 +164,44 @@ let ps_unit =
   {
     parse = (fun _ -> Some ((), 0));
     serialize = (fun _ -> bytes_empty);
-    parse_serialize_inv = (fun _ -> ());
-    serialize_parse_inv = (fun _ -> ());
+    parse_serialize_inv = (fun _ -> bytes_empty_length ());
+    serialize_parse_inv = (fun buf ->
+      bytes_slice_length buf 0 0;
+      bytes_length_zero (bytes_slice buf 0 0)
+    );
     parse_no_lookahead = (fun _ _ -> ());
   }
 
 let ps_lbytes n =
   let parse_lbytes (buf:bytes): option (lbytes n & consumed_length buf) =
-    if Seq.length buf < n then
+    if bytes_length buf < n then
       None
     else
-      Some (Seq.slice buf 0 n, (n <: consumed_length buf))
+      Some (bytes_slice_length buf 0 n;bytes_slice buf 0 n, (n <: consumed_length buf))
   in
   let serialize_lbytes (b:lbytes n): bytes =
     b
   in
+  bytes_empty_length ();
+  assert(parse_lbytes bytes_empty == None);
   {
     parse = parse_lbytes;
     serialize = serialize_lbytes;
-    parse_serialize_inv = (fun x -> ());
+    parse_serialize_inv = (fun x ->
+      bytes_slice_whole x
+    );
     serialize_parse_inv = (fun (buf:bytes) -> ());
     parse_no_lookahead = (fun (b1 b2:bytes) ->
       match parse_lbytes b1 with
       | None -> ()
-      | Some _ -> assert(Seq.equal (Seq.slice b1 0 n) (Seq.slice b2 0 n))
+      | Some _ -> (
+        bytes_slice_slice b1 0 n 0 n;
+        bytes_slice_slice b2 0 n 0 n
+      )
     )
   }
 
+(*
 val ps_uint: t:IT.inttype{IT.unsigned t /\ ~(IT.U1? t)} -> parser_serializer (IT.uint_t t IT.SEC)
 let ps_uint t =
   let nbytes = IT.numbytes t in
@@ -165,6 +217,7 @@ let ps_u16 = ps_uint IT.U16
 let ps_u32 = ps_uint IT.U32
 let ps_u64 = ps_uint IT.U64
 let ps_u128 = ps_uint IT.U128
+*)
 
 (*** Exact parsers ***)
 
@@ -173,7 +226,7 @@ let ps_to_pse #a ps_a =
     match ps_a.parse buf with
     | None -> None
     | Some (x, l) ->
-      if l = Seq.length buf then
+      if l = bytes_length buf then
         Some x
       else
         None
@@ -185,13 +238,16 @@ let ps_to_pse #a ps_a =
     parse_exact = parse_exact_a;
     serialize_exact = serialize_exact_a;
     parse_serialize_inv_exact = (fun x -> ps_a.parse_serialize_inv x);
-    serialize_parse_inv_exact = (fun buf -> ps_a.serialize_parse_inv buf);
+    serialize_parse_inv_exact = (fun buf ->
+      ps_a.serialize_parse_inv buf;
+      bytes_slice_whole buf
+    );
   }
 
 //The two following functions are defined here because F* can't reason on recursive functions defined inside a function
-val _parse_la: #a:Type -> parser_serializer a -> buf:bytes -> Tot (option (list a)) (decreases (Seq.length buf))
+val _parse_la: #a:Type -> parser_serializer a -> buf:bytes -> Tot (option (list a)) (decreases (bytes_length buf))
 let rec _parse_la #a ps_a buf =
-  if Seq.length buf = 0 then (
+  if bytes_length buf = 0 then (
     Some []
   ) else (
     match ps_a.parse buf with
@@ -212,7 +268,7 @@ let rec _serialize_la #a ps_a l =
   match l with
   | [] -> bytes_empty
   | h::t ->
-    Seq.append (ps_a.serialize h) (_serialize_la ps_a t)
+    bytes_concat (ps_a.serialize h) (_serialize_la ps_a t)
 
 #push-options "--fuel 1"
 let pse_list #a ps_a =
@@ -220,21 +276,24 @@ let pse_list #a ps_a =
   let serialize_la (l:list a) = _serialize_la ps_a l in
   let rec parse_serialize_inv_la (l:list a): Lemma (parse_la (serialize_la l) == Some l) =
     match l with
-    | [] -> ()
+    | [] -> bytes_empty_length ()
     | h::t ->
-      if Seq.length (ps_a.serialize h) = 0 then (
+      if bytes_length (ps_a.serialize h) = 0 then (
         ps_a.parse_serialize_inv h;
-        assert (Seq.equal (ps_a.serialize h) bytes_empty)
+        bytes_length_zero (ps_a.serialize h)
       ) else (
-        ps_a.parse_no_lookahead (ps_a.serialize h) (serialize_la (h::t));
+        bytes_concat_length (ps_a.serialize h) (_serialize_la ps_a t);
+        bytes_slice_concat_left (ps_a.serialize h) (_serialize_la ps_a t);
+        bytes_slice_concat_right (ps_a.serialize h) (_serialize_la ps_a t);
         ps_a.parse_serialize_inv h;
-        parse_serialize_inv_la t;
-        assert (Seq.equal (delete_prefix (serialize_la (h::t)) (Seq.length (ps_a.serialize h))) (serialize_la t))
+        bytes_slice_whole (ps_a.serialize h);
+        ps_a.parse_no_lookahead (ps_a.serialize h) (serialize_la (h::t));
+        parse_serialize_inv_la t
       )
   in
-  let rec serialize_parse_inv_la (buf:bytes): Lemma (ensures (match parse_la buf with | None -> True | Some l -> serialize_la l == buf)) (decreases (Seq.length buf)) =
-    if Seq.length buf = 0 then (
-      assert (Seq.equal buf bytes_empty)
+  let rec serialize_parse_inv_la (buf:bytes): Lemma (ensures (match parse_la buf with | None -> True | Some l -> serialize_la l == buf)) (decreases (bytes_length buf)) =
+    if bytes_length buf = 0 then (
+      bytes_length_zero buf
     ) else (
       match parse_la buf with
       | None -> ()
@@ -243,7 +302,7 @@ let pse_list #a ps_a =
         let t = Some?.v (parse_la (delete_prefix buf len)) in
         ps_a.serialize_parse_inv buf;
         serialize_parse_inv_la (delete_prefix buf len);
-        assert (Seq.equal buf (serialize_la l))
+        bytes_concat_slice buf len
     )
   in
   {
@@ -315,7 +374,7 @@ let ps_nat_in_range r =
   }
 
 #push-options "--z3rlimit 20"
-val parser_serializer_exact_to_parser_serializer: #a:Type -> r:size_range -> pse_a:parser_serializer_exact a{forall x. in_range r (Seq.length (pse_a.serialize_exact x))} -> parser_serializer a
+val parser_serializer_exact_to_parser_serializer: #a:Type -> r:size_range -> pse_a:parser_serializer_exact a{forall x. in_range r (bytes_length (pse_a.serialize_exact x))} -> parser_serializer a
 let parser_serializer_exact_to_parser_serializer #a r pse_a =
   let ps_nat = ps_nat_in_range r in
   let parse_a (buf:bytes) =
@@ -323,10 +382,10 @@ let parser_serializer_exact_to_parser_serializer #a r pse_a =
     | None -> None
     | Some (sz, l) -> begin
       let buf2 = delete_prefix buf l in
-      if Seq.length buf2 < sz then (
+      if bytes_length buf2 < sz then (
         None
       ) else (
-        match pse_a.parse_exact (Seq.slice buf2 0 sz) with
+        match pse_a.parse_exact (bytes_slice buf2 0 sz) with
         | None -> None
         | Some x -> Some (x, ((l + sz) <: consumed_length buf))
       )
@@ -334,19 +393,19 @@ let parser_serializer_exact_to_parser_serializer #a r pse_a =
   in
   let serialize_a (x_a:a): bytes =
     let x_serialized = pse_a.serialize_exact x_a in
-    Seq.append (ps_nat.serialize (Seq.length x_serialized)) x_serialized
+    bytes_append (ps_nat.serialize (bytes_length x_serialized)) x_serialized
   in
   {
     parse = parse_a;
     serialize = serialize_a;
     parse_serialize_inv = (fun x ->
       let x_serialized = pse_a.serialize_exact x in
-      let x_sz = Seq.length (x_serialized) in
-      let l = Seq.length (ps_nat.serialize x_sz) in
+      let x_sz = bytes_length (x_serialized) in
+      let l = bytes_length (ps_nat.serialize x_sz) in
       ps_nat.parse_no_lookahead (ps_nat.serialize x_sz) (serialize_a x);
       ps_nat.parse_serialize_inv x_sz;
       pse_a.parse_serialize_inv_exact x;
-      assert (Seq.equal (Seq.slice (delete_prefix (serialize_a x) l) 0 (Seq.length x_serialized)) x_serialized)
+      assert (bytes_equal (bytes_slice (delete_prefix (serialize_a x) l) 0 (bytes_length x_serialized)) x_serialized)
     );
     serialize_parse_inv = (fun (buf:bytes) ->
       match parse_a buf with
@@ -354,8 +413,8 @@ let parser_serializer_exact_to_parser_serializer #a r pse_a =
       | Some (x, l) ->
         let (sz, l) = Some?.v (ps_nat.parse buf) in
         ps_nat.serialize_parse_inv buf;
-        pse_a.serialize_parse_inv_exact (Seq.slice (delete_prefix buf l) 0 sz);
-        assert (Seq.equal (Seq.slice buf 0 (l+sz)) (serialize_a x))
+        pse_a.serialize_parse_inv_exact (bytes_slice (delete_prefix buf l) 0 sz);
+        assert (bytes_equal (bytes_slice buf 0 (l+sz)) (serialize_a x))
     );
     parse_no_lookahead = (fun (b1 b2:bytes) ->
       match parse_a b1 with
@@ -363,7 +422,7 @@ let parser_serializer_exact_to_parser_serializer #a r pse_a =
       | Some (x, len) ->
         ps_nat.parse_no_lookahead b1 b2;
         let (sz, l) = Some?.v (ps_nat.parse b1) in
-        assert (Seq.equal (Seq.slice (delete_prefix b1 l) 0 sz) (Seq.slice (delete_prefix b2 l) 0 sz))
+        assert (bytes_equal (bytes_slice (delete_prefix b1 l) 0 sz) (bytes_slice (delete_prefix b2 l) 0 sz))
     )
   }
 #pop-options
@@ -372,8 +431,8 @@ type bllist (a:Type) (ps_a:parser_serializer a) (r:size_range) = l:list a{in_ran
 
 #push-options "--fuel 1"
 val byte_length_lemma: #a:Type -> ps_a:parser_serializer a -> l:list a -> Lemma
-  (byte_length ps_a l == Seq.length ((pse_list ps_a).serialize_exact l))
-  [SMTPat (Seq.length ((pse_list ps_a).serialize_exact l))]
+  (byte_length ps_a l == bytes_length ((pse_list ps_a).serialize_exact l))
+  [SMTPat (bytes_length ((pse_list ps_a).serialize_exact l))]
 let rec byte_length_lemma #a ps_a l =
   //Why is this needed?
   assert_norm(forall x. (pse_list ps_a).serialize_exact x == _serialize_la ps_a x);
@@ -389,7 +448,7 @@ let ps_list #a r ps_a =
   let pse_bllist_a: parser_serializer_exact (bllist a ps_a r) =
     {
       parse_exact = (fun buf ->
-        if in_range r (Seq.length buf) then
+        if in_range r (bytes_length buf) then
           match pse_la.parse_exact buf with
           | Some x ->
             byte_length_lemma ps_a x;
@@ -412,21 +471,21 @@ let ps_list #a r ps_a =
   parser_serializer_exact_to_parser_serializer r pse_bllist_a
 
 let ps_seq #a r ps_a =
-  FStar.Classical.forall_intro (Seq.lemma_list_seq_bij #a);
-  FStar.Classical.forall_intro (Seq.lemma_seq_list_bij #a);
+  FStar.Classical.forall_intro (bytes_lemma_list_seq_bij #a);
+  FStar.Classical.forall_intro (bytes_lemma_seq_list_bij #a);
   isomorphism
     (blseq a ps_a r)
     (ps_list r ps_a)
-    (fun l -> Seq.seq_of_list l)
-    (fun s -> Seq.seq_to_list s)
+    (fun l -> bytes_seq_of_list l)
+    (fun s -> bytes_seq_to_list s)
 
 #push-options "--fuel 1"
 let ps_bytes r =
-  let rec lemma (b:bytes): Lemma (ensures byte_length ps_u8 (Seq.seq_to_list b) == Seq.length b) (decreases (Seq.length b)) [SMTPat (byte_length ps_u8 (Seq.seq_to_list b))] =
-    if Seq.length b = 0 then (
+  let rec lemma (b:bytes): Lemma (ensures byte_length ps_u8 (bytes_seq_to_list b) == bytes_length b) (decreases (bytes_length b)) [SMTPat (byte_length ps_u8 (bytes_seq_to_list b))] =
+    if bytes_length b = 0 then (
       ()
     ) else (
-      lemma (Seq.slice b 1 (Seq.length b))
+      lemma (bytes_slice b 1 (bytes_length b))
     )
   in
   isomorphism
